adjacent sc: improve config, remove admits 3/n

src/Config.fst
@@ -1,15 +1,19 @@
 module Config
 
-open Prelude
-
 open FStar.Mul
 
+let nb_size_classes = 9sz
+
 inline_for_extraction noextract
-let metadata_max' = 131072ul
+let metadata_max' = 131072UL
+
+module A = Steel.Array
+let _ : squash (US.fits_u64) = A.intro_fits_u64 ()
 
 let metadata_max =
-  US.fits_u32_implies_fits (U32.v page_size * U32.v metadata_max');
-  US.of_u32 metadata_max'
+  US.fits_u64_implies_fits (U32.v page_size * U64.v metadata_max' * US.v nb_size_classes);
+  US.fits_u64_implies_fits (U64.v metadata_max');
+  US.of_u64 metadata_max'
 
 let alg_null = US.v metadata_max + 1
 
