src/Config.fsti
@@ -11,7 +11,16 @@ inline_for_extraction
 let page_size: U32.t = 4096ul
 
 inline_for_extraction
-val metadata_max: v:US.t{US.fits (US.v v * U32.v page_size)}
+val nb_size_classes: v:US.t{
+  US.v v > 0
+}
+
+inline_for_extraction
+val metadata_max: v:US.t{
+  US.v v > 0 /\
+  US.fits (US.v v * U32.v page_size * US.v nb_size_classes) /\
+  US.fits (US.v v * U32.v page_size)
+}
 
 noextract inline_for_extraction
 val alg_null: v:nat{v = US.v metadata_max + 1}
